testdata/out/go/event_gk/event_gk.go
@@ -6,8 +6,6 @@
 package event_gk
 
 import (
-	"github.com/goose-lang/primitive"
-
 	"github.com/tchajed/marshal"
 
 	"github.com/mjschwenne/grackle/testdata/out/go/timestamp_gk"
@@ -16,41 +14,43 @@ import (
 type S struct {
 	Id        uint32
 	Name      string
-	StartTime *timestamp_gk.S
-	EndTime   *timestamp_gk.S
+	StartTime timestamp_gk.S
+	EndTime   timestamp_gk.S
 }
 
-func (e *S) approxSize() uint64 {
-	return 0
-}
-
-func Marshal(e *S, prefix []byte) []byte {
+func Marshal(e S, prefix []byte) []byte {
 	var enc = prefix
 
 	enc = marshal.WriteInt32(enc, e.Id)
 	nameBytes := []byte(e.Name)
 	enc = marshal.WriteInt(enc, uint64(len(nameBytes)))
 	enc = marshal.WriteBytes(enc, nameBytes)
-	primitive.Assume(e.StartTime != nil)
 	enc = timestamp_gk.Marshal(e.StartTime, enc)
-	primitive.Assume(e.EndTime != nil)
 	enc = timestamp_gk.Marshal(e.EndTime, enc)
 
 	return enc
 }
 
-func Unmarshal(s []byte) (*S, []byte) {
-	e := new(S)
+func Unmarshal(s []byte) (S, []byte) {
 	var enc = s // Needed for goose compatibility
+	var id uint32
+	var name string
+	var startTime timestamp_gk.S
+	var endTime timestamp_gk.S
 
-	e.Id, enc = marshal.ReadInt32(enc)
+	id, enc = marshal.ReadInt32(enc)
 	var nameLen uint64
 	var nameBytes []byte
 	nameLen, enc = marshal.ReadInt(enc)
 	nameBytes, enc = marshal.ReadBytesCopy(enc, nameLen)
-	e.Name = string(nameBytes)
-	e.StartTime, enc = timestamp_gk.Unmarshal(enc)
-	e.EndTime, enc = timestamp_gk.Unmarshal(enc)
+	name = string(nameBytes)
+	startTime, enc = timestamp_gk.Unmarshal(enc)
+	endTime, enc = timestamp_gk.Unmarshal(enc)
 
-	return e, enc
+	return S{
+		Id:        id,
+		Name:      name,
+		StartTime: startTime,
+		EndTime:   endTime,
+	}, enc
 }
